divide tests for lia

lia/implications/heap_insert_multi.v
@@ -1,65 +1,9 @@
-Require Import Bool Arith.
 
-Inductive lst : Type :=
-| Nil : lst
-| Cons : nat -> lst -> lst.
+Require Import Bool.
+Require Import Arith.
 
-Inductive heap : Type :=
-| Hleaf : heap
-| Heap : nat -> nat -> heap -> heap -> heap.
-
-Fixpoint right_height (h : heap) : nat :=
-  match h with
-  | Hleaf => 0
-  | Heap k v l r => right_height r + 1
-  end.
-
-Definition rank (h : heap) : nat :=
-  match h with
-  | Hleaf => 0
-  | Heap k v l r => k
-  end.
-
-Fixpoint has_leftist_property (h : heap) : bool :=
-  match h with
-  | Hleaf => true
-  | Heap k v l r =>
-    has_leftist_property l
-    && has_leftist_property r
-    && (right_height r <=? right_height l)
-    && (k =? right_height r + 1)
-  end.
-
-Fixpoint hsize (h : heap) : nat :=
-  match h with
-  | Hleaf => 0
-  | Heap k v l r => hsize l + hsize r + 1
-  end.
-
-Definition mergea (v : nat) (l r : heap) : heap :=
-  if rank r <=? rank l
-    then Heap (rank r + 1) v l r
-    else Heap (rank l + 1) v r l.
-
-Fixpoint merge (h1 : heap) : heap -> heap :=
-  fix merge_aux (h2 : heap) : heap :=
-  match h1, h2 with
-  | h, Hleaf => h
-  | Hleaf, h => h
-  | Heap k1 v1 l1 r1, Heap k2 v2 l2 r2 =>
-    if v2 <? v1
-      then mergea v1 l1 (merge r1 (Heap k2 v2 l2 r2))
-      else mergea v2 l2 (merge_aux r2)
-  end.
-
-Definition hinsert (h : heap) (n : nat) : heap :=
-  merge (Heap 1 n Hleaf Hleaf) h.
-
-Fixpoint hinsert_all (hinsert_all_arg0 : lst) (hinsert_all_arg1 : heap) : heap
-           := match hinsert_all_arg0, hinsert_all_arg1 with
-              | Nil, h => h
-              | Cons n l, h => hinsert (hinsert_all l h) n
-              end.
+Require Import lia_heap_benchmarks.Definitions.
+Require Import lia_heap_benchmarks.Decide.
 
 Lemma rank_right_height : forall h : heap,
   has_leftist_property h = true -> rank h = right_height h.
@@ -89,11 +33,10 @@ Proof.
   - rewrite (rank_right_height r H0) in H1.
     rewrite (rank_right_height l H) in H1.
     simpl. rewrite (rank_right_height l H).
-    apply le_Sn_le in H1.
     apply andb_true_iff. split.
     + apply andb_true_iff. split.
       * rewrite H. rewrite H0. reflexivity.
-      * apply Nat.leb_le. assumption.
+      * apply Nat.leb_le. apply Nat.lt_le_incl. auto.
     + apply Nat.eqb_eq. reflexivity.
 Qed.
 
@@ -125,10 +68,10 @@ Proof.
   - assumption.
 Qed.
 
-Theorem theorem1 : forall (l : lst) (h : heap), eq (has_leftist_property h) true -> eq (has_leftist_property (hinsert_all l h)) true.
+Theorem leftist_hinsert_mulit : forall (l : lst) (h : heap), (has_leftist_property h) = true -> (has_leftist_property (hinsert_all l h)) = true.
 Proof.
   intros.
   induction l.
-  - simpl. assumption.
   - simpl. apply leftist_hinsert. assumption.
+  - simpl. assumption.
 Qed.
