lia/implications/common/Decide.v
@@ -1,0 +1,39 @@
+From QuickChick Require Import QuickChick.
+From lia_heap_benchmarks Require Import Definitions.
+
+Require Import String. Open Scope string.
+
+(* ************************** [ NAT ] *************************** *)
+Derive Show for nat.
+Derive Arbitrary for nat.
+Instance Dec_Eq_nat : Dec_Eq nat.
+Proof. dec_eq. Qed.
+
+(* ************************** [ BOOL ] *************************** *)
+Derive Show for bool.
+Derive Arbitrary for bool.
+Instance Dec_Eq_bool : Dec_Eq bool.
+Proof. dec_eq. Qed.
+
+(* ************************** [ LST ] *************************** *)
+Derive Show for lst.
+Derive Arbitrary for lst.
+Instance Dec_Eq_lst : Dec_Eq lst.
+Proof. dec_eq. Qed.
+
+(* ************************** [ HEAP ] *************************** *)
+Derive Show for heap.
+Derive Arbitrary for heap.
+Instance Dec_Eq_heap : Dec_Eq heap.
+Proof. dec_eq. Qed.
+
+(* ************************** [ OPTION ] *************************** *)
+Instance show_option {T} `{_ : Show T} : Show (option T) := 
+{| show := 
+    let fix aux l :=
+      match l with
+      | None => "None"
+      | Some x => "Some (" ++ show x ++ ")"
+      end
+    in aux
+|}.
