lia/implications/tests/leftist_mergea_by_rank_right_height_2.v
@@ -1,0 +1,44 @@
+From LFindToo Require Import LFindToo.
+
+Require Import Bool.
+Require Import Arith.
+
+Require Import lia_heap_benchmarks.Definitions.
+Require Import lia_heap_benchmarks.Decide.
+
+Lemma rank_right_height : forall h : heap,
+  has_leftist_property h = true -> rank h = right_height h.
+Proof.
+  intros.
+  induction h.
+  - auto.
+  - simpl. simpl in H. apply andb_true_iff in H. destruct H. apply Nat.eqb_eq in H0. assumption.
+Qed.
+
+Lemma leftist_mergea : forall (v : nat) (l r : heap),
+  has_leftist_property l && has_leftist_property r = true
+    -> has_leftist_property (mergea v l r) = true.
+Proof.
+  intros.
+  unfold mergea.
+  apply andb_true_iff in H. destruct H.
+  destruct (Nat.leb_spec (rank r) (rank l)).
+  - rewrite (rank_right_height r H0) in H1.
+  findlemma. Admitted.
+
+    (* rewrite (rank_right_height l H) in H1.
+    simpl. rewrite (rank_right_height r H0).
+    apply andb_true_iff. split.
+    + apply andb_true_iff. split.
+      * rewrite H. rewrite H0. reflexivity.
+      * apply Nat.leb_le. assumption.
+    + apply Nat.eqb_eq. reflexivity.
+  - rewrite (rank_right_height r H0) in H1.
+    rewrite (rank_right_height l H) in H1.
+    simpl. rewrite (rank_right_height l H).
+    apply andb_true_iff. split.
+    + apply andb_true_iff. split.
+      * rewrite H. rewrite H0. reflexivity.
+      * apply Nat.leb_le. apply Nat.lt_le_incl. auto.
+    + apply Nat.eqb_eq. reflexivity.
+Qed. *)
