vfa_selection/tests/cons_of_small_maintains_sort_by_le_all__le_one.v
@@ -1,3 +1,17 @@
+(** * Selection:  Selection Sort *)
+(* Some proofs from: https://github.com/kolya-vasiliev/verified-functional-algorithms-2019/blob/master/Selection.v *)
+
+From LFindToo Require Import LFindToo.
+
+Require Import vfa_selection_benchmarks.Definitions.
+Require Import vfa_selection_benchmarks.Decide.
+
+(* These specify the libraries of functions that should be considered during synthesis that 
+    are not defined within the above libraries. *)
+Require Import Coq.Lists.List.
+Require Import Coq.Sorting.Permutation. 
+
+(* ################################################################# *)
 
 Lemma cons_of_small_maintains_sort: forall bl y n,
   n = length bl -> y <=* bl -> sorted (selsort bl n) -> sorted (y :: selsort bl n).
